<?xml version="1.0"?>


<!DOCTYPE rdf:RDF [
    <!ENTITY owl "http://www.w3.org/2002/07/owl#" >
    <!ENTITY dc "http://purl.org/dc/elements/1.1/" >
    <!ENTITY xsd "http://www.w3.org/2001/XMLSchema#" >
    <!ENTITY skos "http://www.w3.org/2004/02/skos/core#" >
    <!ENTITY xml "http://www.w3.org/XML/1998/namespace" >
    <!ENTITY rdfs "http://www.w3.org/2000/01/rdf-schema#" >
    <!ENTITY rdf "http://www.w3.org/1999/02/22-rdf-syntax-ns#" >
    <!ENTITY metadata-annotations "http://purl.org/ninepts/metadata/metadata-annotations#" >
]>


<rdf:RDF xmlns="http://purl.org/ninepts/metadata/metadata-annotations#"
     xml:base="http://purl.org/ninepts/metadata/metadata-annotations"
     xmlns:dc="http://purl.org/dc/elements/1.1/"
     xmlns:rdfs="http://www.w3.org/2000/01/rdf-schema#"
     xmlns:metadata-annotations="http://purl.org/ninepts/metadata/metadata-annotations#"
     xmlns:owl="http://www.w3.org/2002/07/owl#"
     xmlns:xsd="http://www.w3.org/2001/XMLSchema#"
     xmlns:rdf="http://www.w3.org/1999/02/22-rdf-syntax-ns#"
     xmlns:xml="http://www.w3.org/XML/1998/namespace"
     xmlns:skos="http://www.w3.org/2004/02/skos/core#">
    <owl:Ontology rdf:about="http://purl.org/ninepts/metadata/metadata-annotations">
        <license rdf:datatype="&xsd;anyURI">http://opensource.org/licenses/MIT</license>
        <anotherFormat rdf:datatype="&xsd;anyURI">http://purl.org/ninepts/metadata/metadata-annotations.ofn</anotherFormat>
        <rdfs:seeAlso rdf:datatype="&xsd;anyURI">http://purl.org/ninepts/metadata/metadata-properties.owl</rdfs:seeAlso>
        <mimeType>application/rdf+xml</mimeType>
        <dateCreated>2014-04-16</dateCreated>
        <skos:changeNote xml:lang="en">28 April 2014
* Updated the URIs of the widely deployed Dublin Core and SKOS concepts to use the DC and SKOS URIs 
** Updated URIs are: contributor, coverage, creator, date, description, language, relation, rights, *Label, note, *Note
* Removed the definition property (since description can be used), the coverage properties (since their semantics are not precise and keywords are available), and the usageNote property (since scopeNote could be used instead)
* Completed the metadata details of the remaining properties
* Added altLabel_Plural and prefLabel_Plural properties, and competencyQuestions and competencyQuery properties
* Renamed the property, replaces, to replacementFor
* Moved exactMatch to be a sub-property of closeMatch, as defined by SKOS</skos:changeNote>
        <keyword xml:lang="en">Dublin Core</keyword>
        <skos:prefLabel xml:lang="en">Metadata Ontology (Using Annotation Properties)</skos:prefLabel>
        <dc:description xml:lang="en">Ontology providing a small, basic set of metadata concepts, based on Dublin Core and SKOS.  The concepts are defined as annotation properties.</dc:description>
        <competencyQuery>PREFIX rdf: &lt;http://www.w3.org/1999/02/22-rdf-syntax-ns#&gt; 
PREFIX owl: &lt;http://www.w3.org/2002/07/owl#&gt; 
PREFIX skos: &lt;http://www.w3.org/2004/02/skos/core#&gt; 
SELECT ?s ?work WHERE { 
   ?s skos:editorialNote ?work . 
}
# What work remains to be done on the ontology, and what decisions still need to be made?</competencyQuery>
        <skos:changeNote xml:lang="en">01 May 2014
* Corrected the predicate of one of the competencyQueries (was mislabeled as competencyQuestions)</skos:changeNote>
        <competencyQuery>SELECT ?p ?o WHERE { 
   &lt;http://purl.org/ninepts/metadata/metadata-annotations&gt; ?p ?o . 
}
# What metadata information is available for the ontology?</competencyQuery>
        <dateLastModified>2014-05-07</dateLastModified>
        <skos:scopeNote xml:lang="en">It is important to note that not all concepts are included from the Dublin Core or SKOS sources.  Where the concepts overlap with established semantics in RDF or OWL 2, they are not repeated. A list of the omitted concepts is provided below.

Also note that where the concepts overlap in Dublin Core and SKOS, only one annotation property is created.  (But the mappingRelation properties will indicate both mappings.) An example of this is the correspondence between Dublin Core&apos;s title and SKOS&apos; prefLabel.

What follows is a list of the Dublin Core Elements vocabulary and SKOS model concepts that are not included in this ontology (and why):

 - DC:coverage (spatial/temporal topic) - Coverage is of limited use because it is not restricted with respect to vocabulary or temporal/spatial format.  Also, one cannot know if the value defines a topic, applicability or jurisdiction. Time and location will be defined as separate ontologies with more precise semantics.  
 - DC:format (file and mime formats) - Can be achieved using the mimeType property. 
 - DC:identifier (unambiguous reference) - The URI of an entity provides this reference.
 - DC:publisher - The source of the ontology may be determined from its IRI, copyright, or similar properties.  Typically, an ontology is made available on a web site, installed with software, etc. and is copyrighted. 
 - DC:source - The mappingRelation sub-properties (taken from SKOS) provide more explicit information regarding the source/origin of an ontology or its components.
 - DC:type (DCMI Type) - DCMI types include software, images, etc. and MIME types.  Instead of the general DCMI type, a mimeType property is defined.
 - SKOS:Concept (unit of thought) - A class definition with its metadata corresponds to a Concept.
 - SKOS:ConceptScheme and inScheme (collection of concepts) - An ontology (and its namespace) collects related concepts.
 - SKOS:Collection, OrderedCollection, member, memberList - Will be defined in a separate ontology dealing specifically with the Collection semantic.
 - SKOS:definition - Use the dc: description property instead.
 - SKOS:hasTopConcept and topConceptOf (defines the top Concept in a ConceptScheme) - Can be achieved by subclassing from owl:Top for an ontology.
 - SKOKS:notation - Can be achieved by defining a new data type and referencing it in a value or as the range of a data property.
 - SKOS:semanticRelation, related, broader, narrower, broaderTransitive, narrowerTransitive - Can be achieved using subclassing.  The related semantic is equivalent to an owl SymmetricProperty.
 - SKOS:relatedMatch - Can be achieved by using the mappingRelation property (and not the more specific sub-properties).

</skos:scopeNote>
        <competencyQuery>PREFIX rdf: &lt;http://www.w3.org/1999/02/22-rdf-syntax-ns#&gt; 
PREFIX owl: &lt;http://www.w3.org/2002/07/owl#&gt; 
PREFIX skos: &lt;http://www.w3.org/2004/02/skos/core#&gt; 
SELECT ?s ?change WHERE { 
   ?s skos:changeNote ?change . 
}
# How has the ontology evolved? What changes have been documented in the ontology?</competencyQuery>
        <competencyQuery>PREFIX rdf: &lt;http://www.w3.org/1999/02/22-rdf-syntax-ns#&gt; 
PREFIX owl: &lt;http://www.w3.org/2002/07/owl#&gt; 
SELECT ?metadata WHERE { 
   ?metadata rdf:type owl:AnnotationProperty . 
   FILTER ( 
      regex(str(?metadata), &quot;skos/core&quot;) || regex(str(?metadata), &quot;dc/elements&quot;) 
   ) 
}
# How do the metadata properties correspond/map to the Dublin Core and SKOS concepts?  Specifically, what Dublin Core and SKOS values are directly defined/used in the ontology?</competencyQuery>
        <competencyQuery>PREFIX rdf: &lt;http://www.w3.org/1999/02/22-rdf-syntax-ns#&gt; 
PREFIX owl: &lt;http://www.w3.org/2002/07/owl#&gt; 
PREFIX skos: &lt;http://www.w3.org/2004/02/skos/core#&gt; 
SELECT ?metadata WHERE { 
    ?metadata rdf:type owl:AnnotationProperty . 
   OPTIONAL {
      ?metadata skos:example ?example . 
   } . 
   FILTER ( 
      !bound(?example) 
   ) 
}
# What metadata properties in the ontology have no example?</competencyQuery>
        <competencyQuery>PREFIX rdf: &lt;http://www.w3.org/1999/02/22-rdf-syntax-ns#&gt; 
PREFIX owl: &lt;http://www.w3.org/2002/07/owl#&gt; 
PREFIX dc: &lt;http://purl.org/dc/elements/1.1/&gt; 
SELECT ?metadata ?description WHERE { 
   ?metadata rdf:type owl:AnnotationProperty . 
   ?metadata dc:description ?description . 
}
# What is the meaning/semantic of each of the metadata properties?</competencyQuery>
        <competencyQuery>PREFIX rdf: &lt;http://www.w3.org/1999/02/22-rdf-syntax-ns#&gt; 
PREFIX owl: &lt;http://www.w3.org/2002/07/owl#&gt; 
SELECT ?metadata ?mapping ?stdConcept WHERE { 
   ?metadata rdf:type owl:AnnotationProperty . 
   ?metadata ?mapping ?stdConcept . 
   FILTER ( 
      regex(str(?mapping), &quot;closeMatch&quot;) || regex(str(?mapping), &quot;exactMatch&quot;) || 
      regex(str(?mapping), &quot;inspiredBy&quot;) || regex(str(?mapping), &quot;moreGeneralThan&quot;) ||  
      regex(str(?mapping), &quot;moreSpecificThan&quot;) 
   ) . 
   FILTER ( 
      regex(str(?stdConcept), &quot;skos/core&quot;) || regex(str(?stdConcept), &quot;dc/elements&quot;) 
   ) 
}
# How do the metadata properties correspond/map to the Dublin Core and SKOS concepts?  Specifically, are there any mappings of metadata properties to Dublin Core and SKOS concepts?</competencyQuery>
        <competencyQuery>PREFIX rdf: &lt;http://www.w3.org/1999/02/22-rdf-syntax-ns#&gt; 
PREFIX owl: &lt;http://www.w3.org/2002/07/owl#&gt; 
PREFIX meta: &lt;http://purl.org/ninepts/metadata/metadata-annotations#&gt;
SELECT ?query WHERE { 
   ?s meta:competencyQuery ?query . 
}
# What queries should be run to validate the ontology?</competencyQuery>
        <dc:creator>Andrea Westerinen
Nine Points Solutions, LLC</dc:creator>
        <owl:priorVersion>0.5.0</owl:priorVersion>
        <skos:changeNote xml:lang="en">07 May 2014
* Description property for moreSpecificThan should have been an example property
* Updated examples for the relation properties
* Updated all the competencyQueries (correcting the syntax)</skos:changeNote>
        <copyright xml:lang="en">Copyright (c) 2014 Nine Points Solutions, LLC</copyright>
        <competencyQuery>PREFIX rdf: &lt;http://www.w3.org/1999/02/22-rdf-syntax-ns#&gt; 
PREFIX owl: &lt;http://www.w3.org/2002/07/owl#&gt; 
PREFIX dc: &lt;http://purl.org/dc/elements/1.1/&gt; 
SELECT ?metadata WHERE { 
    ?metadata rdf:type owl:AnnotationProperty . 
   OPTIONAL {
      ?metadata dc:description ?description . 
   } . 
   FILTER ( 
      !bound(?description) 
   ) 
}
# What metadata properties in the ontology have no description?</competencyQuery>
        <keyword xml:lang="en">SKOS</keyword>
        <license xml:lang="en">The MIT License (MIT)

Copyright (c) 2014 Nine Points Solutions, LLC

Permission is hereby granted, free of charge, to any person obtaining a copy
of this software and associated documentation files (the &quot;Software&quot;), to deal
in the Software without restriction, including without limitation the rights
to use, copy, modify, merge, publish, distribute, sublicense, and/or sell
copies of the Software, and to permit persons to whom the Software is
furnished to do so, subject to the following conditions:

The above copyright notice and this permission notice shall be included in
all copies or substantial portions of the Software.

THE SOFTWARE IS PROVIDED &quot;AS IS&quot;, WITHOUT WARRANTY OF ANY KIND, EXPRESS OR
IMPLIED, INCLUDING BUT NOT LIMITED TO THE WARRANTIES OF MERCHANTABILITY,
FITNESS FOR A PARTICULAR PURPOSE AND NONINFRINGEMENT. IN NO EVENT SHALL THE
AUTHORS OR COPYRIGHT HOLDERS BE LIABLE FOR ANY CLAIM, DAMAGES OR OTHER
LIABILITY, WHETHER IN AN ACTION OF CONTRACT, TORT OR OTHERWISE, ARISING FROM,
OUT OF OR IN CONNECTION WITH THE SOFTWARE OR THE USE OR OTHER DEALINGS IN
THE SOFTWARE.</license>
        <skos:scopeNote xml:lang="en">This ontology is intended to be usable/imported to any ontology to provide basic metadata for provenance and reuse. It is designed to be independent of any specific domain.

NOTE: When querying or hand-editing this ontology (or one that imports this ontology), take care to use the correct namespace for the properties.  The base URI is http://purl.org/ninepts/metadata/metadata-annotations#.  The namespaces, http://purl.org/dc/elements/1.1/ and http://www.w3.org/2004/02/skos/core#, are also used.

Issues with the ontology may be entered and tracked at http://github.com/NinePts/reusable-ontologies/.</skos:scopeNote>
        <dc:language>en-US</dc:language>
        <competencyQuery>PREFIX rdf: &lt;http://www.w3.org/1999/02/22-rdf-syntax-ns#&gt; 
PREFIX owl: &lt;http://www.w3.org/2002/07/owl#&gt; 
PREFIX skos: &lt;http://www.w3.org/2004/02/skos/core#&gt; 
SELECT ?metadata ?scope WHERE { 
   ?metadata rdf:type owl:AnnotationProperty . 
   ?metadata skos:scopeNote ?scope . 
}
# Are there any restrictions or suggestions for the use of the various metadata properties?</competencyQuery>
        <competencyQuestions xml:lang="en">* What metadata information is available for the ontology?
* What is the meaning/semantic of each of the metadata properties?
* What is an example of the use of each of the metadata properties?
* Are there any restrictions or suggestions for the use of the various metadata properties?
* How do the metadata properties correspond/map to the Dublin Core and SKOS concepts?
* How has the ontology evolved? What changes have been documented in the ontology?
* What work remains to be done on the ontology, and what decisions still need to be made?
* What queries should be run to validate the ontology?
* What metadata properties have no description or no example?</competencyQuestions>
        <competencyQuery>PREFIX rdf: &lt;http://www.w3.org/1999/02/22-rdf-syntax-ns#&gt; 
PREFIX owl: &lt;http://www.w3.org/2002/07/owl#&gt; 
PREFIX skos: &lt;http://www.w3.org/2004/02/skos/core#&gt; 
SELECT ?metadata ?example WHERE { 
   ?metadata rdf:type owl:AnnotationProperty . 
   ?metadata skos:example ?example . 
}
# What is an example of the use of each of the metadata properties?</competencyQuery>
        <rdfs:comment xml:lang="en">This ontology is a consolidation of basic metadata concepts from the Dublin Core Element and Terms vocabularies, and the SKOS data model.  The semantics are captured as annotation properties.  

Where the concepts are widely deployed from Dublin Core and SKOS, the property names use the full URIs from those sources.  For example, the property name of &quot;description&quot; is the Dublin Core URI, http://purl.org/dc/elements/1.1/description, and does not use this ontology&apos;s namespace.  This allows tooling that &quot;understands&quot; the standard terms (like description or SKOS&apos; prefLabel) to immediately recognize (and appropriately present) the concepts.

Note that the ontology referenced using the seeAlso property (http://purl.org/ninepts/metadata/metadata-properties.ofn) defines several of the  annotation properties as data and object properties.  This allows (for example) validating  dateTime values and referencing objects/individuals in relations (as opposed to using literal values). </rdfs:comment>
        <keyword xml:lang="en">metadata</keyword>
        <owl:versionIRI rdf:resource="http://purl.org/ninepts/metadata/metadata-annotations/0.6.0"/>
    </owl:Ontology>
    


    <!-- 
    ///////////////////////////////////////////////////////////////////////////////////////
    //
    // Annotation properties
    //
    ///////////////////////////////////////////////////////////////////////////////////////
     -->

    


    <!-- http://purl.org/dc/elements/1.1/contributor -->

    <owl:AnnotationProperty rdf:about="&dc;contributor">
        <dc:description xml:lang="en">An entity responsible for making contributions to an ontology, class, property or individual.</dc:description>
        <skos:example xml:lang="en">Andrea Westerinen (a person&apos;s name)</skos:example>
        <rdfs:comment xml:lang="en">Examples of a contributor include a person, an organization or a service. Typically, the name of a contributor should be used to indicate the entity.</rdfs:comment>
        <skos:example xml:lang="en">Nine Points Solutions, LLC (a company/organization name)</skos:example>
        <skos:scopeNote xml:lang="en">This property is intended to be used at the level of the ontology, although a specific class, property or individual may be labeled with a contributor.</skos:scopeNote>
        <skos:prefLabel xml:lang="en">contributor</skos:prefLabel>
        <prefLabel_Plural xml:lang="en">contributors</prefLabel_Plural>
    </owl:AnnotationProperty>
    


    <!-- http://purl.org/dc/elements/1.1/creator -->

    <owl:AnnotationProperty rdf:about="&dc;creator">
        <dc:description xml:lang="en">An entity responsible for initially defining the ontology, class, property or individual.</dc:description>
        <skos:example xml:lang="en">Andrea Westerinen (a person&apos;s name)</skos:example>
        <rdfs:comment xml:lang="en">Examples of a creator include a person, an organization or a service. Typically, the name of a creator should be used to indicate the entity.</rdfs:comment>
        <skos:example xml:lang="en">Nine Points Solutions, LLC (a company/organization name)</skos:example>
        <skos:scopeNote xml:lang="en">This property is intended to be used at the level of the ontology, although a specific class, property or individual may be labeled with a creator.</skos:scopeNote>
        <skos:prefLabel xml:lang="en">creator</skos:prefLabel>
        <prefLabel_Plural xml:lang="en">creators</prefLabel_Plural>
    </owl:AnnotationProperty>
    


    <!-- http://purl.org/dc/elements/1.1/date -->

    <owl:AnnotationProperty rdf:about="&dc;date">
        <skos:example rdf:datatype="&xsd;dateTime">2014-05-21T07:33:03</skos:example>
        <skos:example>2014-05-21</skos:example>
        <dc:description xml:lang="en">A point or period of time associated with an event in the lifecycle of the ontology.</dc:description>
        <rdfs:comment xml:lang="en">Date may be used to express temporal information at any level of granularity.  Recommended best practice is to use an encoding scheme, such as the W3CDTF profile of ISO 8601.</rdfs:comment>
        <skos:scopeNote xml:lang="en">Use of this property is not recommended.  Instead, use one of its subproperties since they define explicit semantics and format.

When defining dates for individuals, it is recommended that a data property be used.  The corresponding data property is defined in the metadata-properties ontology.

Note that the date/time format defined by Dublin Core is not a valid date/time datatype in OWL 2.  The Dublin Core date/time information would have to be converted to the OWL format, or imported as an OWL literal.</skos:scopeNote>
        <skos:prefLabel xml:lang="en">date</skos:prefLabel>
        <prefLabel_Plural xml:lang="en">dates</prefLabel_Plural>
    </owl:AnnotationProperty>
    


    <!-- http://purl.org/dc/elements/1.1/description -->

    <owl:AnnotationProperty rdf:about="&dc;description">
        <closeMatch rdf:datatype="&xsd;anyURI">http://www.w3.org/2004/02/skos/core#definition</closeMatch>
        <dc:description xml:lang="en">An explanation of an ontology, concept, property or individual.  Descriptions are typically longer forms of definitions and/or elaborate on a definition.</dc:description>
        <skos:example xml:lang="en">An explanation of the meaning of a concept, the characteristics or information about an individual, etc.</skos:example>
        <rdfs:comment xml:lang="en">Description may include but is not limited to an abstract, a graphical representation, a free-text account, etc.</rdfs:comment>
        <skos:scopeNote xml:lang="en">If desired, a definition annotation property may also be created, although that is not done in this ontology.</skos:scopeNote>
        <skos:prefLabel xml:lang="en">description</skos:prefLabel>
        <prefLabel_Plural xml:lang="en">descriptions</prefLabel_Plural>
    </owl:AnnotationProperty>
    


    <!-- http://purl.org/dc/elements/1.1/language -->

    <owl:AnnotationProperty rdf:about="&dc;language">
        <dc:description xml:lang="en">The (natural) language in which the ontology, class, property or individual is expressed.</dc:description>
        <skos:example>en-US</skos:example>
        <rdfs:comment xml:lang="en">Recommended best practice is to use a controlled vocabulary such as defined in IETF RFC 4646.</rdfs:comment>
        <skos:scopeNote xml:lang="en">When applied to an ontology, the property defines the primary language used to specify the classes, properties and individuals.  Note that some classes, properties and individuals may be specified in another language, and will carry their own language annotation.  Also, a XML language attribute may be added to any literal value.

Language values must follow the syntax defined in IETF RFC 4646.  The RFC is available at http://www.ietf.org/rfc/rfc4646.txt.</skos:scopeNote>
        <skos:prefLabel xml:lang="en">language</skos:prefLabel>
        <prefLabel_Plural xml:lang="en">languages</prefLabel_Plural>
    </owl:AnnotationProperty>
    


    <!-- http://purl.org/dc/elements/1.1/relation -->

    <owl:AnnotationProperty rdf:about="&dc;relation">
        <dc:description xml:lang="en">A reference to a related entity.</dc:description>
        <skos:example xml:lang="en">ISBN reference</skos:example>
        <rdfs:comment xml:lang="en">Recommended best practice is to identify the related resource by means of a string conforming to a formal identification system.</rdfs:comment>
        <skos:scopeNote xml:lang="en">Use of this property is not recommended.  Instead, use of one of its subproperties is recommended since those properties define explicit semantics and format.</skos:scopeNote>
        <skos:prefLabel xml:lang="en">relation</skos:prefLabel>
        <prefLabel_Plural xml:lang="en">relations</prefLabel_Plural>
        <skos:example xml:lang="en">text_includingURI_defining_someRelatedEntity</skos:example>
    </owl:AnnotationProperty>
    


    <!-- http://purl.org/dc/elements/1.1/rights -->

    <owl:AnnotationProperty rdf:about="&dc;rights">
        <skos:example xml:lang="en">Digital rights, licensing, copyright details as text</skos:example>
        <dc:description xml:lang="en">Information about the entitlements held in and over the ontology.</dc:description>
        <skos:scopeNote xml:lang="en">It is assumed that the rights property (and its sub-properties) only apply at the ontology level.

Although the property could be applied to any OWL construct, it is discouraged to use it at the class, property or  individual level.  Having different rights for entities within the ontology (different from the rights defined at the ontology level) may result in misuse of the information.  It is recommended that entities with different rights be placed in different ontologies and different ontology files.</skos:scopeNote>
        <rdfs:comment xml:lang="en">Typically, rights information includes a statement about various property rights associated with the ontology, including intellectual property rights.</rdfs:comment>
        <prefLabel_Plural xml:lang="en">rights</prefLabel_Plural>
        <skos:prefLabel xml:lang="en">rights</skos:prefLabel>
    </owl:AnnotationProperty>
    


    <!-- http://purl.org/ninepts/metadata/metadata-annotations#altLabel_Plural -->

    <owl:AnnotationProperty rdf:about="&metadata-annotations;altLabel_Plural">
        <skos:example xml:lang="en">Alternate Labels (versus the prefLabel_Plural, Alternative Labels)</skos:example>
        <skos:scopeNote xml:lang="en">Plural forms of altLabels are not needed for single valued/functional properties (since each entity will only have 1 value for the property), or the name/title of an individual.

Note that the plural form of an altLabel can be specified simply as an altLabel.  But, this is confusing when choosing/displaying labels, and pluralization is not always simple.  For this reason, the plural forms of alternative labels are recommended to be placed in a specific property, altLabel_Plural.

Since relationships between annotation property values cannot be defined, it is not possible to define the correspondence between the singular and plural forms of a label.</skos:scopeNote>
        <dc:description xml:lang="en">The (optional) plural form of an altLabel, in a given natural language, useful for human-readable representations.  The alternatives may be synonyms, acronyms, abbreviations, spelling variations, etc.</dc:description>
        <skos:altLabel xml:lang="en">alternate label (plural)</skos:altLabel>
        <altLabel_Plural xml:lang="en">alternate labels (plurals)</altLabel_Plural>
        <skos:prefLabel xml:lang="en">alternative label (plural)</skos:prefLabel>
        <prefLabel_Plural xml:lang="en">alternative labels (plurals)</prefLabel_Plural>
        <rdfs:subPropertyOf rdf:resource="&rdfs;label"/>
    </owl:AnnotationProperty>
    


    <!-- http://purl.org/ninepts/metadata/metadata-annotations#anotherFormat -->

    <owl:AnnotationProperty rdf:about="&metadata-annotations;anotherFormat">
        <moreSpecificThan rdf:datatype="&xsd;anyURI">http://purl.org/dc/elements/1.1/relation</moreSpecificThan>
        <exactMatch rdf:datatype="&xsd;anyURI">http://purl.org/dc/terms/hasFormat</exactMatch>
        <skos:example xml:lang="en">More specific example:
http://some_namespace/ontology-es.ofn (defined for an ontology written in English for a version of an ontology rendered using Spanish as the native language)</skos:example>
        <skos:example xml:lang="en">More specific example:
http://some_namespace/ontology.rdf (defined for an ontology serialized in Turtle, referencing the ontology serialized using RDF/XML)</skos:example>
        <skos:scopeNote xml:lang="en">Note that this relationship can be interpreted as transitive.</skos:scopeNote>
        <dc:description xml:lang="en">References an ontology, class, property or individual that is substantially the same as the subject of this relation, but in another format.</dc:description>
        <skos:prefLabel xml:lang="en">another format</skos:prefLabel>
        <prefLabel_Plural xml:lang="en">other formats</prefLabel_Plural>
        <skos:example xml:lang="en">text_includingURI_defining_someExample</skos:example>
        <rdfs:subPropertyOf rdf:resource="&dc;relation"/>
    </owl:AnnotationProperty>
    


    <!-- http://purl.org/ninepts/metadata/metadata-annotations#closeMatch -->

    <owl:AnnotationProperty rdf:about="&metadata-annotations;closeMatch">
        <moreSpecificThan rdf:datatype="&xsd;anyURI">http://purl.org/dc/elements/1.1/relation</moreSpecificThan>
        <exactMatch rdf:datatype="&xsd;anyURI">http://www.w3.org/2004/02/skos/core#closeMatch</exactMatch>
        <skos:scopeNote xml:lang="en">Note that this relationship is NOT considered to be transitive.</skos:scopeNote>
        <dc:description xml:lang="en">References an ontology, class, property or individual that is &quot;sufficiently similar&quot; as to be used interchangeably.  The match only has meaning in applications that are aware of both the subject and object of the relationship, and should not be interpreted as transitive.</dc:description>
        <skos:prefLabel xml:lang="en">close match</skos:prefLabel>
        <skos:example xml:lang="en">text_includingURI_defining_someSimilarEntity</skos:example>
        <rdfs:subPropertyOf rdf:resource="&metadata-annotations;mappingRelation"/>
    </owl:AnnotationProperty>
    


    <!-- http://purl.org/ninepts/metadata/metadata-annotations#competencyQuery -->

    <owl:AnnotationProperty rdf:about="&metadata-annotations;competencyQuery">
        <dc:description xml:lang="en">A translation of a competency question to SPARQL.  The query can be run to validate an ontology.</dc:description>
        <skos:scopeNote xml:lang="en">Competency questions and corresponding queries are defined for ontologies, and are not associated with classes, properties or individuals.

Each query should be specified in individual competencyQuery triples.</skos:scopeNote>
        <skos:example xml:lang="en">SELECT * WHERE {?s ?p ?o}</skos:example>
        <prefLabel_Plural xml:lang="en">competency queries</prefLabel_Plural>
        <skos:prefLabel xml:lang="en">competency query</skos:prefLabel>
    </owl:AnnotationProperty>
    


    <!-- http://purl.org/ninepts/metadata/metadata-annotations#competencyQuestions -->

    <owl:AnnotationProperty rdf:about="&metadata-annotations;competencyQuestions">
        <dc:description xml:lang="en">Competency questions (per the 1995 paper by Gruninger and Fox) are &quot;requirements that are in the form of questions that [the] ontology must be able to answer.&quot;  The questions can be translated to queries and help to define the scope of the ontology.</dc:description>
        <skos:scopeNote xml:lang="en">Competency questions are defined for ontologies, and are not associated with classes, properties or individuals.

Whereas the query corresponding to each question is defined in different competencyQuery triples, there should be only one triple defined with the competencyQuestions predicate.</skos:scopeNote>
        <skos:example xml:lang="en">The following competency questions are taken from the Ontology Development 101 web page  (http://protege.stanford.edu/publications/ontology_development/ontology101-noy-mcguinness.html), &quot;Step 1. Determine the domain and scope of the ontology&quot; for a food and wine ontology:
* Which wine characteristics should I consider when choosing a wine?
* Is Bordeaux a red or white wine?
* Does Cabernet Sauvignon go well with seafood?
* What is the best choice of wine for grilled meat?
* Does a bouquet or body of a specific wine change with vintage year?
* What were good vintages for Napa Zinfandel?</skos:example>
        <skos:prefLabel xml:lang="en">competency questions</skos:prefLabel>
        <prefLabel_Plural xml:lang="en">competency questions</prefLabel_Plural>
    </owl:AnnotationProperty>
    


    <!-- http://purl.org/ninepts/metadata/metadata-annotations#copyright -->

    <owl:AnnotationProperty rdf:about="&metadata-annotations;copyright">
        <moreSpecificThan rdf:datatype="&xsd;anyURI">http://purl.org/dc/elements/1.1/rights</moreSpecificThan>
        <skos:example xml:lang="en">Copyright (c) 2014, Nine Points Solutions, LLC</skos:example>
        <skos:scopeNote xml:lang="en">It is assumed that the copyright property only applies at the ontology level.

Although the property could be applied to any OWL construct, it is discouraged to use it at the class, property or  individual level.  Having different copyrights for entities within the ontology (different from the rights defined at the ontology level) may result in misuse of the information.  It is recommended that entities with different copyrights be placed in different ontologies and different ontology files.</skos:scopeNote>
        <dc:description xml:lang="en">The copyright statement for an ontology.  Per WordNet, copyright is &quot;the exclusive legal right, given to an originator or an assignee to print, publish, perform, film, or record literary, artistic, or musical material, and to authorize others to do the same.&quot;</dc:description>
        <skos:prefLabel xml:lang="en">copyright</skos:prefLabel>
        <prefLabel_Plural xml:lang="en">copyrights</prefLabel_Plural>
        <rdfs:subPropertyOf rdf:resource="&dc;rights"/>
    </owl:AnnotationProperty>
    


    <!-- http://purl.org/ninepts/metadata/metadata-annotations#dateCreated -->

    <owl:AnnotationProperty rdf:about="&metadata-annotations;dateCreated">
        <closeMatch rdf:datatype="&xsd;anyURI"> http://purl.org/dc/terms/created</closeMatch>
        <skos:example rdf:datatype="&xsd;dateTime">2014-04-14T12:45:00</skos:example>
        <moreSpecificThan rdf:datatype="&xsd;anyURI">http://purl.org/dc/elements/1.1/date</moreSpecificThan>
        <skos:example>2014-04-14</skos:example>
        <dc:description xml:lang="en">The point or period of time (for example, the year) when the ontology, class, property or individual was created.</dc:description>
        <skos:scopeNote xml:lang="en">This property is intended to be used at any level of the ontology, including defining the date when a particular class, property or individual was created. Use of a data property is recommended for individuals (for example, to record when a trouble ticket was reported/created).  The corresponding data property is defined in the metadata-properties ontology.

In Dublin Core, values of the created date property use the format defined by the W3CDTF profile of ISO 8601.  However, that format is not a valid date/time datatype in OWL 2.  The Dublin Core date/time created information would have to be converted to the OWL format, or imported as an OWL literal.  For this reason, the Dublin Core property is mapped as a &quot;close&quot; and not an &quot;exact&quot; match.</skos:scopeNote>
        <skos:prefLabel xml:lang="en">date created</skos:prefLabel>
        <rdfs:subPropertyOf rdf:resource="&dc;date"/>
    </owl:AnnotationProperty>
    


    <!-- http://purl.org/ninepts/metadata/metadata-annotations#dateLastModified -->

    <owl:AnnotationProperty rdf:about="&metadata-annotations;dateLastModified">
        <skos:example rdf:datatype="&xsd;dateTime">2014-04-28T23:52:00</skos:example>
        <moreSpecificThan rdf:datatype="&xsd;anyURI">http://purl.org/dc/terms/modified</moreSpecificThan>
        <skos:example>2014-04-28</skos:example>
        <dc:description xml:lang="en">A point or period of time (for example, the year) when the ontology, class, property or individual was last modified.</dc:description>
        <skos:scopeNote xml:lang="en">This property is intended to be used at any level of the ontology, including defining the date when a particular class, property or individual was last modified. Use of a data property is recommended for individuals (for example, to record when a trouble ticket was last updated).  The corresponding data property is defined in the metadata-properties ontology.

If a set of modification dates is needed, as opposed to recording the date of the last change, use the dateModified property.

Note that in Dublin Core, values of the modified date property use the format defined by the W3CDTF profile of ISO 8601.  However, that format is not a valid date/time datatype in OWL 2.  The Dublin Core date/time modified information would have to be converted to the OWL format, or imported as an OWL literal.  </skos:scopeNote>
        <skos:prefLabel xml:lang="en">date last modified</skos:prefLabel>
        <moreSpecificThan xml:lang="en">http://purl.org/dc/elements/1.1/date</moreSpecificThan>
        <rdfs:subPropertyOf rdf:resource="&metadata-annotations;dateModified"/>
    </owl:AnnotationProperty>
    


    <!-- http://purl.org/ninepts/metadata/metadata-annotations#dateModified -->

    <owl:AnnotationProperty rdf:about="&metadata-annotations;dateModified">
        <skos:example rdf:datatype="&xsd;dateTime">2014-04-16T17:12:00</skos:example>
        <moreSpecificThan rdf:datatype="&xsd;anyURI">http://purl.org/dc/elements/1.1/date</moreSpecificThan>
        <closeMatch rdf:datatype="&xsd;anyURI">http://purl.org/dc/terms/modified</closeMatch>
        <skos:example>2014-04-16</skos:example>
        <dc:description xml:lang="en">A point or period of time (for example, the year) when the ontology, class, property or individual was modified.</dc:description>
        <skos:scopeNote xml:lang="en">This property is intended to be used at any level of the ontology, including defining the date when a particular class, property or individual was modified. Use of a data property is recommended for individuals (for example, to record when a trouble ticket was updated).  The corresponding data property is defined in the metadata-properties ontology.

If a set of modification dates is not valuable, but only knowing the date of the last modification, use the dateLastModified property.

In Dublin Core, values of the modified date property use the format defined by the W3CDTF profile of ISO 8601.  However, that format is not a valid date/time datatype in OWL 2.  The Dublin Core date/time modified information would have to be converted to the OWL format, or imported as an OWL literal.  For this reason, the Dublin Core property is mapped as a &quot;close&quot; and not an &quot;exact&quot; match.</skos:scopeNote>
        <skos:prefLabel xml:lang="en">date modified</skos:prefLabel>
        <prefLabel_Plural xml:lang="en">dates modified</prefLabel_Plural>
        <rdfs:subPropertyOf rdf:resource="&dc;date"/>
    </owl:AnnotationProperty>
    


    <!-- http://purl.org/ninepts/metadata/metadata-annotations#exactMatch -->

    <owl:AnnotationProperty rdf:about="&metadata-annotations;exactMatch">
        <moreSpecificThan rdf:datatype="&xsd;anyURI">http://purl.org/dc/elements/1.1/relation</moreSpecificThan>
        <exactMatch rdf:datatype="&xsd;anyURI">http://www.w3.org/2004/02/skos/core#exactMatch</exactMatch>
        <skos:scopeNote xml:lang="en">Note that this relation is considered to be transitive.</skos:scopeNote>
        <dc:description xml:lang="en">References a semantically similar ontology, class, property or individual.  ExactMatch indicates that the two entities have equivalent semantics, and can be used interchangeably.  By definition, this is a transitive relationship.</dc:description>
        <skos:prefLabel xml:lang="en">exact match</skos:prefLabel>
        <skos:example xml:lang="en">text_includingURI_defining_someEquivalentEntity</skos:example>
        <rdfs:subPropertyOf rdf:resource="&metadata-annotations;closeMatch"/>
    </owl:AnnotationProperty>
    


    <!-- http://purl.org/ninepts/metadata/metadata-annotations#inspiredBy -->

    <owl:AnnotationProperty rdf:about="&metadata-annotations;inspiredBy">
        <moreSpecificThan rdf:datatype="&xsd;anyURI">http://purl.org/dc/elements/1.1/relation</moreSpecificThan>
        <skos:example xml:lang="en">ISBN reference (to publication containing basic concepts)</skos:example>
        <dc:description xml:lang="en">References some entity which inspired the definition of the subject of the relationship.  The referenced entity could be of similar scope and definition (for example, a class in one ontology inspiring the definition of class or property in another ontology), or completely different (for example, Aristotle&apos;s classifications providing the basis for an &quot;upper&quot; ontology).</dc:description>
        <skos:prefLabel xml:lang="en">inspired by</skos:prefLabel>
        <skos:example xml:lang="en">text_includingURI_defining_someSource</skos:example>
        <rdfs:subPropertyOf rdf:resource="&metadata-annotations;mappingRelation"/>
    </owl:AnnotationProperty>
    


    <!-- http://purl.org/ninepts/metadata/metadata-annotations#keyword -->

    <owl:AnnotationProperty rdf:about="&metadata-annotations;keyword">
        <moreSpecificThan rdf:datatype="&xsd;anyURI">http://purl.org/dc/elements/1.1/subject</moreSpecificThan>
        <dc:description xml:lang="en">A word or phrase that describes the ontology, class, property or individual.</dc:description>
        <skos:scopeNote xml:lang="en">The keyword can be a single word or a word phrase.  The terms can be open-ended or come from a controlled vocabulary.</skos:scopeNote>
        <skos:example xml:lang="en">a_keyword phrase (multi-word phrase)</skos:example>
        <skos:example xml:lang="en">a_keyword_for_the_entity</skos:example>
        <skos:prefLabel xml:lang="en">keyword</skos:prefLabel>
        <prefLabel_Plural xml:lang="en">keywords</prefLabel_Plural>
    </owl:AnnotationProperty>
    


    <!-- http://purl.org/ninepts/metadata/metadata-annotations#license -->

    <owl:AnnotationProperty rdf:about="&metadata-annotations;license">
        <skos:example rdf:datatype="&xsd;anyURI">http://opensource.org/licenses/MIT</skos:example>
        <moreSpecificThan rdf:datatype="&xsd;anyURI">http://purl.org/dc/elements/1.1/rights</moreSpecificThan>
        <exactMatch rdf:datatype="&xsd;anyURI">http://purl.org/dc/terms/license</exactMatch>
        <skos:example xml:lang="en">Multiple types of open-source licenses can be browsed at http://opensource.org/licenses.</skos:example>
        <dc:description xml:lang="en">The licensing applied to the ontology.  A license is a legal document giving official permission to do something with the ontology.</dc:description>
        <skos:scopeNote xml:lang="en">The specific wording of the license (or a reference to a location where the wording can be found) should be provided as the value of this property.  Note that both the wording AND the reference can be provided (since the former allows the license to be available offline). 

It is assumed that the license property only applies at the ontology level.

Although the property could be applied to any OWL construct, it is discouraged to use it at the class, property or  individual level.  Having different licenses for entities within the ontology (different from the licenses defined at the ontology level) may result in misuse of the information.  It is recommended that entities with different licenses be placed in different ontologies and different ontology files.</skos:scopeNote>
        <skos:prefLabel xml:lang="en">license</skos:prefLabel>
        <prefLabel_Plural xml:lang="en">licenses</prefLabel_Plural>
        <rdfs:subPropertyOf rdf:resource="&dc;rights"/>
    </owl:AnnotationProperty>
    


    <!-- http://purl.org/ninepts/metadata/metadata-annotations#mappingRelation -->

    <owl:AnnotationProperty rdf:about="&metadata-annotations;mappingRelation">
        <moreSpecificThan rdf:datatype="&xsd;anyURI">http://purl.org/dc/elements/1.1/relation</moreSpecificThan>
        <exactMatch rdf:datatype="&xsd;anyURI">http://www.w3.org/2004/02/skos/core#mappingRelation</exactMatch>
        <skos:scopeNote xml:lang="en">It is recommended that one of the sub-properties of mappingRelation be used to describe the specific semantics of the mapping.  This property is too general (under-specified) to be useful.</skos:scopeNote>
        <dc:description xml:lang="en">References an ontology, class, property or individual which can be mapped to the subject of the relationship.</dc:description>
        <skos:prefLabel xml:lang="en">mapping relation</skos:prefLabel>
        <prefLabel_Plural xml:lang="en">mapping relations</prefLabel_Plural>
        <skos:example xml:lang="en">text_includingURI_defining_someMappedEntity</skos:example>
        <rdfs:subPropertyOf rdf:resource="&dc;relation"/>
    </owl:AnnotationProperty>
    


    <!-- http://purl.org/ninepts/metadata/metadata-annotations#mimeType -->

    <owl:AnnotationProperty rdf:about="&metadata-annotations;mimeType">
        <moreSpecificThan rdf:datatype="&xsd;anyURI">http://purl.org/dc/elements/1.1/format</moreSpecificThan>
        <moreSpecificThan rdf:datatype="&xsd;anyURI">http://purl.org/dc/elements/1.1/type</moreSpecificThan>
        <skos:scopeNote xml:lang="en">This property is intended to be used at the level of the ontology, to define the serialization format in which the ontology was/is encoded.  There is only one serialization format per file.

Note that when the ontology is loaded into a tool or data store, the serialization format is no longer relevant.

Possible values of MIME type for OWL ontologies are:
 - text/owl-functional (extension .ofn)
 - text/owl-manchester (extension .omn)
 - application/owl+xml (extension .owx)
 - application/rdf+xml (extension .rdf)
 - text/turtle (extension .ttl)

These values are taken from the IANA Media Type definitions, available at 
http://www.iana.org/assignments/media-types/media-types.xhtml.</skos:scopeNote>
        <skos:example>text/owl-functional</skos:example>
        <dc:description xml:lang="en">The MIME type of the ontology, as defined by the various OWL 2 syntaxes in their W3C Recommendations, and as assigned by IANA.
</dc:description>
        <skos:prefLabel xml:lang="en">mime type</skos:prefLabel>
        <prefLabel_Plural xml:lang="en">mime types</prefLabel_Plural>
    </owl:AnnotationProperty>
    


    <!-- http://purl.org/ninepts/metadata/metadata-annotations#moreGeneralThan -->

    <owl:AnnotationProperty rdf:about="&metadata-annotations;moreGeneralThan">
        <moreSpecificThan rdf:datatype="&xsd;anyURI">http://purl.org/dc/elements/1.1/relation</moreSpecificThan>
        <closeMatch rdf:datatype="&xsd;anyURI">http://www.w3.org/2004/02/skos/core#narrowMatch</closeMatch>
        <closeMatch rdf:datatype="&xsd;anyURI">http://www.w3.org/2004/02/skos/core#narrower</closeMatch>
        <dc:description xml:lang="en">References some entity that is a more specific concept than the subject of the relationship (i.e., the subject would be considered to be a super-type/super-property of the object).</dc:description>
        <skos:scopeNote xml:lang="en">Typically, moreGeneralThan is used to relate class and property concepts, and not ontologies or individuals.  The relationship is particularly useful when merging/mapping ontologies, vocabularies, etc., in order to place the concepts in a subsumption hierarchy.

Note that this relation can be considered to be transitive.  That is why it is only defined as a &quot;closeMatch&quot; to the SKOS concepts of narrowMatch and narrower.  (In the SKOS model, these two relations are not guaranteed to be transitive.)</skos:scopeNote>
        <skos:prefLabel xml:lang="en">more general than</skos:prefLabel>
        <skos:example xml:lang="en">text_includingURI_defining_someMoreSpecificEntity</skos:example>
        <rdfs:subPropertyOf rdf:resource="&metadata-annotations;mappingRelation"/>
    </owl:AnnotationProperty>
    


    <!-- http://purl.org/ninepts/metadata/metadata-annotations#moreSpecificThan -->

    <owl:AnnotationProperty rdf:about="&metadata-annotations;moreSpecificThan">
        <moreSpecificThan rdf:datatype="&xsd;anyURI">http://purl.org/dc/elements/1.1/relation</moreSpecificThan>
        <closeMatch rdf:datatype="&xsd;anyURI">http://www.w3.org/2004/02/skos/core#broadMatch</closeMatch>
        <closeMatch rdf:datatype="&xsd;anyURI">http://www.w3.org/2004/02/skos/core#broader</closeMatch>
        <dc:description xml:lang="en">References some entity that is a more general concept than the subject of the relationship (i.e., the subject would be considered to be a sub-type/sub-property of the object).</dc:description>
        <skos:scopeNote xml:lang="en">Typically, moreSpecificThan is used to relate class and property concepts, and not ontologies or individuals.  The relationship is particularly useful when merging/mapping ontologies, vocabularies, etc., in order to place the concepts in a subsumption hierarchy.

Note that this relation can be considered to be transitive.  That is why it is only defined as a &quot;closeMatch&quot; to the SKOS concepts of broadMatch and broader.  (In the SKOS model, these two relations are not guaranteed to be transitive.)</skos:scopeNote>
        <skos:prefLabel xml:lang="en">more specific than</skos:prefLabel>
        <skos:example xml:lang="en">text_includingURI_defining_someMoreGeneralEntity</skos:example>
        <rdfs:subPropertyOf rdf:resource="&metadata-annotations;mappingRelation"/>
    </owl:AnnotationProperty>
    


    <!-- http://purl.org/ninepts/metadata/metadata-annotations#prefLabel_Plural -->

    <owl:AnnotationProperty rdf:about="&metadata-annotations;prefLabel_Plural">
        <skos:example xml:lang="en">Preferred Labels (versus the prefLabel, Preferred Label)</skos:example>
        <dc:description xml:lang="en">The (optional) plural form of prefLabel for an entity, in a given natural language, useful for human-readable representations.  There is only one plural form of a preferred label per language for an entity.</dc:description>
        <skos:scopeNote xml:lang="en">There is only one plural form of the preferred label per language for an entity.

The plural form of a prefLabel is not needed for single valued/functional properties (since each entity will only have 1 value for the property), or the name/title of an individual.</skos:scopeNote>
        <skos:prefLabel xml:lang="en">preferred label (plural)</skos:prefLabel>
        <prefLabel_Plural xml:lang="en">preferred labels (plurals)</prefLabel_Plural>
        <rdfs:subPropertyOf rdf:resource="&rdfs;label"/>
    </owl:AnnotationProperty>
    


    <!-- http://purl.org/ninepts/metadata/metadata-annotations#replacementFor -->

    <owl:AnnotationProperty rdf:about="&metadata-annotations;replacementFor">
        <moreSpecificThan rdf:datatype="&xsd;anyURI">http://purl.org/dc/elements/1.1/relation</moreSpecificThan>
        <exactMatch rdf:datatype="&xsd;anyURI">http://purl.org/dc/terms/replaces</exactMatch>
        <skos:example xml:lang="en">More specific example:
http://some_namespace/ontology_v1.ofn (defined for v2 of an ontology, referencing a version which it replaces)</skos:example>
        <dc:description xml:lang="en">References an ontology, class, property or individual that is supplanted, displaced or superceded by the subject of the relation.</dc:description>
        <skos:scopeNote xml:lang="en">The replacementFor relation can be used in many different scenarios- for example, to describe the wholesale evolution of an ontology or individual (such as a document/specification), or to describe how a class or property definition evolves over time.  In the case of the latter, a class or property could be deprecated (using the owl#deprecated annotation property), and a new entity defined that is a &quot;replacementFor&quot; it.

Note that the relation can be interpreted as transitive.</skos:scopeNote>
        <skos:prefLabel xml:lang="en">replacement for</skos:prefLabel>
        <skos:example xml:lang="en">text_includingURI_defining_someDeprecatedOrOlderEntity</skos:example>
        <rdfs:subPropertyOf rdf:resource="&dc;relation"/>
    </owl:AnnotationProperty>
    


    <!-- http://www.w3.org/2000/01/rdf-schema#comment -->

    <rdf:Description rdf:about="&rdfs;comment">
        <skos:prefLabel xml:lang="en">comment</skos:prefLabel>
        <prefLabel_Plural xml:lang="en">comments</prefLabel_Plural>
    </rdf:Description>
    


    <!-- http://www.w3.org/2000/01/rdf-schema#label -->

    <rdf:Description rdf:about="&rdfs;label">
        <skos:prefLabel xml:lang="en">label</skos:prefLabel>
        <prefLabel_Plural xml:lang="en">labels</prefLabel_Plural>
    </rdf:Description>
    


    <!-- http://www.w3.org/2002/07/owl#priorVersion -->

    <rdf:Description rdf:about="&owl;priorVersion">
        <skos:prefLabel xml:lang="en">prior version</skos:prefLabel>
        <prefLabel_Plural xml:lang="en">prior versions</prefLabel_Plural>
    </rdf:Description>
    


    <!-- http://www.w3.org/2004/02/skos/core#altLabel -->

    <owl:AnnotationProperty rdf:about="&skos;altLabel">
        <dc:description xml:lang="en">A alternative label for an entity, in a given natural language, useful for human-readable representations.  The alternative may be a synonym, acronym/abbreviation, spelling variation, etc.</dc:description>
        <skos:example xml:lang="en">Alternate Label (versus the prefLabel, Alternative Label)</skos:example>
        <skos:scopeNote xml:lang="en">Note that a plural form of a prefLabel or altLabel is allowed as the property&apos;s value.  But, this is confusing when choosing/displaying labels.  For this reason, the plural form of prefLabel and alternative labels are recommended to be placed in specific properties, prefLabel_Plural and altLabel_Plural, respectively.</skos:scopeNote>
        <skos:altLabel xml:lang="en">alternate label</skos:altLabel>
        <altLabel_Plural xml:lang="en">alternate labels</altLabel_Plural>
        <skos:prefLabel xml:lang="en">alternative label</skos:prefLabel>
        <prefLabel_Plural xml:lang="en">alternative labels</prefLabel_Plural>
        <rdfs:subPropertyOf rdf:resource="&rdfs;label"/>
    </owl:AnnotationProperty>
    


    <!-- http://www.w3.org/2004/02/skos/core#changeNote -->

    <owl:AnnotationProperty rdf:about="&skos;changeNote">
        <skos:example xml:lang="en">(change note for an ontology) 
01-May-2014 
* Added properties, ABC and XYZ
* Updated the description of the class, foo</skos:example>
        <dc:description xml:lang="en">Documents fine-grained changes to an ontology, class, property or individual, for the purposes of administration and maintenance.</dc:description>
        <skos:scopeNote xml:lang="en">It may be easiest to capture all changes to an ontology in a single change note (which is updated with each evolution of the ontology), or one can use multiple notes (one for each evolution).  However, if desired, any specific change to a class, property or individual may be described using this property.</skos:scopeNote>
        <skos:prefLabel xml:lang="en">change note</skos:prefLabel>
        <prefLabel_Plural xml:lang="en">change notes</prefLabel_Plural>
        <rdfs:subPropertyOf rdf:resource="&skos;note"/>
    </owl:AnnotationProperty>
    


    <!-- http://www.w3.org/2004/02/skos/core#editorialNote -->

    <owl:AnnotationProperty rdf:about="&skos;editorialNote">
        <dc:description xml:lang="en">Documents information for an ontology, class, property or individual that aids administrative housekeeping, such as reminders of editorial work still to be done, or warnings in the event that future editorial changes might be made.</dc:description>
        <skos:example xml:lang="en">Review the viability of this property after the decision regarding XYZ is complete.</skos:example>
        <skos:prefLabel xml:lang="en">editorial note</skos:prefLabel>
        <prefLabel_Plural xml:lang="en">editorial notes</prefLabel_Plural>
        <rdfs:subPropertyOf rdf:resource="&skos;note"/>
    </owl:AnnotationProperty>
    


    <!-- http://www.w3.org/2004/02/skos/core#example -->

    <owl:AnnotationProperty rdf:about="&skos;example">
        <dc:description xml:lang="en">Describes an example of a class individual or a property value.</dc:description>
        <skos:scopeNote xml:lang="en">Examples are relevant for classes and properties, but not for ontologies and individuals.</skos:scopeNote>
        <skos:example xml:lang="en">For a class, Person, the individual AndreaWesterinen is an example.</skos:example>
        <skos:example xml:lang="en">For a dateCreated property, the value &quot;23-Apr-2014&quot;^^xsd:dateTime is an example.</skos:example>
        <skos:prefLabel xml:lang="en">example</skos:prefLabel>
        <prefLabel_Plural xml:lang="en">examples</prefLabel_Plural>
        <rdfs:subPropertyOf rdf:resource="&skos;note"/>
    </owl:AnnotationProperty>
    


    <!-- http://www.w3.org/2004/02/skos/core#hiddenLabel -->

    <owl:AnnotationProperty rdf:about="&skos;hiddenLabel">
        <dc:description xml:lang="en">A label for an entity, in a given natural language, that is not displayed to any users, but which may be used in queries.  For example, mis-spelled words may be values of this property - which are useful for search but should not be considered as viable labels.</dc:description>
        <skos:example xml:lang="en">Hiden Label (misspelling of the prefLabel, Hidden Label)</skos:example>
        <skos:prefLabel xml:lang="en">hidden label</skos:prefLabel>
        <prefLabel_Plural xml:lang="en">hidden labels</prefLabel_Plural>
        <rdfs:subPropertyOf rdf:resource="&rdfs;label"/>
    </owl:AnnotationProperty>
    


    <!-- http://www.w3.org/2004/02/skos/core#note -->

    <owl:AnnotationProperty rdf:about="&skos;note">
        <skos:example xml:lang="en">A note can be documentation of a change, for an editor, providing an example, defining how a concept is used, etc.</skos:example>
        <dc:description xml:lang="en">Human-readable documentation of an ontology, class, property or individual.</dc:description>
        <skos:scopeNote xml:lang="en">It is not recommended to use the generic note property, but to use one of the more specific subproperties.  

Note that rdfs:comment and dc:description properties also may be used for documentation.</skos:scopeNote>
        <skos:prefLabel xml:lang="en">note</skos:prefLabel>
        <prefLabel_Plural xml:lang="en">notes</prefLabel_Plural>
    </owl:AnnotationProperty>
    


    <!-- http://www.w3.org/2004/02/skos/core#prefLabel -->

    <owl:AnnotationProperty rdf:about="&skos;prefLabel">
        <moreSpecificThan rdf:datatype="&xsd;anyURI">http://purl.org/dc/elements/1.1/title</moreSpecificThan>
        <skos:example xml:lang="en">Preferred Label</skos:example>
        <dc:description xml:lang="en">The preferred label or title for an entity, in a given natural language, useful for human-readable representations.  There is only one preferred label per language for an entity.</dc:description>
        <skos:scopeNote xml:lang="en">There is only one preferred label per language for an entity.</skos:scopeNote>
        <skos:prefLabel xml:lang="en">preferred label</skos:prefLabel>
        <prefLabel_Plural xml:lang="en">preferred labels</prefLabel_Plural>
        <rdfs:subPropertyOf rdf:resource="&rdfs;label"/>
    </owl:AnnotationProperty>
    


    <!-- http://www.w3.org/2004/02/skos/core#scopeNote -->

    <owl:AnnotationProperty rdf:about="&skos;scopeNote">
        <dc:description xml:lang="en">Provides additional documentation (beyond the description) on the meaning or use of the ontology, class, property or individual.</dc:description>
        <skos:example xml:lang="en">This concept should be/should not be used in the following scenarios: ...</skos:example>
        <skos:prefLabel xml:lang="en">scope note</skos:prefLabel>
        <prefLabel_Plural xml:lang="en">scope notes</prefLabel_Plural>
        <rdfs:subPropertyOf rdf:resource="&skos;note"/>
    </owl:AnnotationProperty>
</rdf:RDF>



<!-- Generated by the OWL API (version 3.4.2) http://owlapi.sourceforge.net -->

